---
layout: default
title: "Reading notes for Modern Particle Physics, Mark Thomson (Chapter 4)"
date: 2025-8-6
categories: [particle physics]
tags: [reading notes, particle physics]
---

## Chapter 4 The Dirac equation

### The Klein-Gordon Equation

The naïve thought of the K-G equation:

the energy-mass equation:
$$
E^2 = p^2+m^2
$$
To change this equation into wave equation, let $E \to \mathrm i \frac{\partial }{\partial t}$, $ p \to -\mathrm i \nabla$, hence
$$
\left(\frac{\partial ^2}{\partial t^2}-\nabla^2+m^2\right)\psi = 0
$$
i.e.,
$$
(\partial^\mu\partial_\mu+m^2)\psi =0
$$
In order to obtain the probability density and probability current of this wave function, consider
$$
\psi^*\frac{\partial^2}{\partial t^2}\psi = \psi^*(\nabla^2-m^2)\psi\\
\psi\frac{\partial^2}{\partial t^2}\psi^* = \psi(\nabla^2-m^2)\psi^*
$$
Take the subtraction of these 2 equations above, we get
$$
\frac{\partial}{\partial t}\mathrm i(\psi^*\frac{\partial \psi}{\partial t}-\psi\frac{\partial \psi^*}{\partial t})-\nabla \cdot \mathrm i(\psi^*\nabla\psi -\psi\nabla\psi^*)=0
$$
For freedom wave function, we have
$$
\psi = N\mathrm e^{\mathrm i (\vec p \cdot \vec x-Et)}
$$

$$
\rho =\mathrm i(\psi^*\frac{\partial \psi}{\partial t}-\psi\frac{\partial \psi^*}{\partial t})=2|N|^2E\\
\vec j = -\mathrm i(\psi^*\nabla\psi -\psi\nabla\psi^*)= 2|N|^2\vec p
$$

Obviously when E<0, the probability density comes to be below zero, which sounds ridiculous for physicists.

### The Dirac Equation

To limit the wave function to that gives the positive probability density, Dirac tried to constrain the equation into 1-partial-derivation, i.e.,
$$
\mathrm i \frac{\partial}{\partial t}\psi = (\vec \alpha \cdot \hat {\vec p} +\beta m)\psi = (-\mathrm i\vec \alpha\cdot\nabla+\beta m )\psi
$$
Apparently this function needs to accommodate with the energy-mass equation, i.e.
$$
\left(\mathrm i \frac{\partial}{\partial t}\right)\cdot\left(\mathrm i \frac{\partial}{\partial t}\right)\psi = (-\mathrm i\vec \alpha\cdot\nabla+\beta m )\cdot (-\mathrm i\vec \alpha\cdot\nabla+\beta m )\psi= (p^2+m^2)\psi
$$
Hence,
$$
\alpha_x^2= \alpha_y^2=\alpha_z^2=\beta^2 = 1\\
\alpha_i\beta+\beta\alpha_i=0,i = x, y, z\\
\alpha_i\alpha_j+\alpha_j\alpha_i = 0, i, j = x, y ,z, i \neq j
$$
To satisfy the algebra above, we have
$$
\alpha_i = 
\begin{bmatrix}
0 & \sigma_i \\
\sigma_i & 0
\end{bmatrix}, \quad
\beta = 
\begin{bmatrix}
I & 0 \\
0 & -I
\end{bmatrix}
$$
where $\sigma_i$ is one of Pauli matrices.

### Probability density and probability current

Similar to the calculation of the K-G equation, we have
$$
\psi^\dagger\left(\mathrm i \frac{\partial}{\partial t}\right)\psi = \psi^\dagger(-\mathrm i\vec \alpha\cdot\nabla+\beta m )\psi\\
\left(-\mathrm i \frac{\partial}{\partial t}\right)\psi^\dagger\psi = (\mathrm i\vec \alpha\cdot\nabla+\beta m )\psi^\dagger\psi
$$
Take the subtraction of these 2 equations above, we gain
$$
\frac{\partial}{\partial t}(\psi^\dagger\psi) +\nabla\cdot(\psi^\dagger\vec\alpha\psi)=0
$$

i.e.,
$$
\rho = \psi^\dagger\psi,\vec j = \psi^\dagger\vec \alpha\psi
$$


---

### Spin and the Dirac Equation

(TO BE CONTINUED)

---

### Covariant form of the Dirac Equation

The Dirac equation:
$$
\mathrm i \frac{\partial}{\partial t}\psi = (-\mathrm i \vec \alpha\cdot\nabla+\beta m)\psi
$$
Multiply this by $\beta$, we have
$$
(\mathrm i\gamma^\mu\partial_\mu-m)\psi= 0
$$
where
$$
\gamma_0 =\beta, \gamma_i = \beta\alpha_i
$$
We regard this **as** the covariant form of the Dirac equation, albeit with the constant factor gamma. One step more, we get the transformer rule for the Dirac spinor. 

#### The adjoint spinor and the covariant current

For $\vec j^\mu =(\rho, \vec j)$,
$$
\vec j = \psi^\dagger\vec \alpha\psi= \psi^\dagger\beta\beta\alpha\psi=\psi^\dagger\gamma^0\gamma^\mu\psi=\bar \psi\gamma^\mu\psi
$$
where $\bar\psi = \psi^\dagger\gamma^0$, called adjoint spinor. This operation is also suitable for probability density.

### Solutions to the Dirac equation

Scenario #1: particle with zero momentum

Dirac Eq.:
$$
\mathrm i \frac{\partial}{\partial t}\psi = (-\mathrm i \alpha\cdot\nabla+\beta m)\psi
$$
With $\psi = u\mathrm e^{-\mathrm i Et}$, we have
$$
Eu\mathrm e^{-\mathrm i Et}=
\begin{bmatrix}
I & 0 \\
0 & -I
\end{bmatrix}
m u\mathrm e^{-\mathrm i Et}
$$
i.e.,
$$
\begin{bmatrix}
-m & 0 \\
0 & m
\end{bmatrix}
\begin{bmatrix}
U_1\\
U_2
\end{bmatrix}
=
E
\begin{bmatrix}
U_1\\
U_2
\end{bmatrix}
$$
For eigen value $E_+= m$ (the energy-mass equation), we have 
$$
u_1=
\begin{bmatrix}
1\\
0\\
0\\
0
\end{bmatrix}, \quad
u_2=
\begin{bmatrix}
0\\
1\\
0\\
0
\end{bmatrix}
$$
For eigen value $E_-=-m$ (the energy-mass equation), we have
$$
u_3=
\begin{bmatrix}
0\\
0\\
1\\
0
\end{bmatrix}, \quad
u_4=
\begin{bmatrix}
0\\
0\\
0\\
1
\end{bmatrix}
$$
Thus 
$$
u = A_1u_1+A_2u_2+A_3u_3+A_4u_4
$$
Scenario #2: particle with momentum $p$ in direction z.

Dirac Eq.:
$$
\mathrm i \frac{\partial}{\partial t}\psi = (-\mathrm i \alpha\cdot\nabla+\beta m)\psi
$$
With $\psi = u\mathrm e^{\mathrm i (\vec p\cdot \vec x-Et)}$, we have
$$
\begin{bmatrix}
m & \sigma\cdot p \\
\sigma\cdot p & -m
\end{bmatrix}
\begin{bmatrix}
U_1\\
U_2
\end{bmatrix}
=
E
\begin{bmatrix}
U_1\\
U_2
\end{bmatrix}
$$

> Useful equation:
> $$
> (\sigma\cdot \vec A)(\sigma \cdot \vec B)=\sigma_iA_i\sigma_jb_j=\sigma_i\sigma_ja_ib_j= a_ib_i+\mathrm i \epsilon_{ijk}\sigma_ka_ib_j = \vec A \cdot \vec B + \sigma \cdot(\vec A\times\vec B)
> $$

Solving the eigen value equation, we have
$$
\det \begin{bmatrix}
m-E & \sigma\cdot p \\
\sigma\cdot p & -m-E
\end{bmatrix} 
= E^2-m^2-p^2=0
$$

Thus $E_1= \sqrt{p^2+m^2}, E_2 = -\sqrt{p^2+m^2}$, $U_1 = \frac{1}{E-m}\sigma\cdot pU_2, U_2 = \frac{1}{E+m}\sigma\cdot p U_1$.

Therefore for eigen value $E_1= \sqrt{p^2+m^2}$, 
$$
u_1=
\begin{bmatrix}
1\\
0\\
\frac{1}{E_1+m}p_z\\
\frac{1}{E_1+m}(p_x-\mathrm i p_y)
\end{bmatrix}, \quad
u_2=
\begin{bmatrix}
0\\
1\\
\frac{1}{E_1+m}(p_x+\mathrm i p_y)\\
-\frac{1}{E_1+m}p_z
\end{bmatrix}
$$
Therefore for eigen value $E_2 = -\sqrt{p^2+m^2}$, 
$$
u_3=
\begin{bmatrix}
\frac{1}{E_2-m}p_z\\
\frac{1}{E_2-m}(p_x-\mathrm i p_y)\\
1\\
0\\
\end{bmatrix}, \quad
u_4=
\begin{bmatrix}
\frac{1}{E_2-m}(p_x+\mathrm i p_y)\\
-\frac{1}{E_2-m}p_z\\
0\\
1\\
\end{bmatrix}
$$

$$
u = A_1u_1+A_2u_2+A_3u_3+A_4u_4
$$

### Antiparticles

For physics reason, we **have to** get proper explanation for these negative energy. 

#### The Dirac sea interpretation

To be concise, Dirac thought the negative energy levels are **almost completely occupied**, so the particle cannot reach these negative energy levels due to the Pauli's exclusion principle. When a vacant position with negative energy appears, the positive-energy particle (the normal kind) jump into the hole in the negative Dirac sea, and release energy.

#### The Feynman-Stückelberg  interpretation

---

(TO BE CONTINUED)

the confusion for propagate backwards in time

---

### Antiparticle spinors

For negative wavefunctions that propagate backwards in time, we can extract the negative sign from E and p, which is
$$
v(E, \vec p)\mathrm e^{-\mathrm i (\vec p \cdot \vec x -Et)}= u(-E, -\vec p)\mathrm e ^{\mathrm i ((-\vec p)\cdot \vec x -(-E)t)}
$$
To satisfy the Dirac function, we get the Lorentz-invariant form of this equation, 
$$
(\gamma^\mu p_\mu+m)v = 0
$$

$$
\begin{bmatrix}
E+m &-\sigma \cdot p\\
\sigma \cdot p & -E+m\\
\end{bmatrix}
\begin{bmatrix}
V_1\\
V_2\\
\end{bmatrix}= 0
$$

$$
V_1 = \frac{\sigma\cdot p}{E+m}V_2, V_2 = \frac{\sigma\cdot p}{E-m}V_1
$$

Note that the positive eigen value E corresponds to the "normal" wavefunction with negative function. 

So we have 
$$
v_1 = \begin{bmatrix}
\frac{p_x-\mathrm i p_y}{E+m}\\
\frac{-p_z}{E+m}\\
0\\
1\\
\end{bmatrix}, \quad
v_2 = \begin{bmatrix}
\frac{p_z}{E+m}\\
\frac{p_x+\mathrm i p_y}{E+m}\\
1\\
0\\
\end{bmatrix}
$$
for E > 0 and 
$$
v_3=
\begin{bmatrix}
1\\
0\\
\frac{p_z}{E-m}\\
\frac{p_x+\mathrm i p_y}{E-m}
\end{bmatrix}, \quad
v_4=
\begin{bmatrix}
0\\
1\\
\frac{p_x-\mathrm i p_y}{E-m}\\
\frac{-p_z}{E-m}\\
\end{bmatrix}
$$
for E < 0.

With the equivalence of u-function and v-function, we can construct the genal wave function with $(u_1, u_2, v_1, v_2)$.

According to the normalization rule for wave function$\psi^\dagger\psi = 2E$, we have 
$$
u(v)_{1(2)}^*= \sqrt{E+m}\, u(v)_{1(2)}
$$

#### Operators and the antiparticle spinors  

Just remember that for antiparticle wavefunction, the physical energy and momentum are given by
$$
H^{(v)}= -\mathrm i\partial _t, p^{(v)}=\mathrm i \nabla
$$

### Charge conjugation  

---

(TO BE CONTINUED)

---

### Spin and helicity states

The z-axis 'spin matrix'
$$
S_z = \frac{1}{2}
\begin{bmatrix}
\sigma_z & 0\\
0 &-\sigma_z
\end{bmatrix}
$$
apparently not commute with the Dirac Hamiltonian.

To solve this problem, we construct a new concept called helicity, which is
$$
h = \frac{S\cdot p}{p} =\frac{1}{2p} 
\begin{bmatrix}
\sigma \cdot p & 0\\
0 & \sigma \cdot p 
\end{bmatrix}
$$
This physical quantity can be commute with the Dirac Hamiltonian, and can help degenerate the eigen vectors for H.

Consider the eigen vector u for h,
$$
\frac{1}{2p} 
\begin{bmatrix}
\sigma \cdot p & 0\\
0 & \sigma \cdot p 
\end{bmatrix}
\begin{bmatrix}
U_1\\
U_2
\end{bmatrix}
= \lambda
\begin{bmatrix}
U_1\\
U_2
\end{bmatrix}
$$

$$
\frac{1}{2p}\sigma\cdot p \, U_{1, 2}= \lambda U_{1, 2}
$$

Apparently $\lambda = \pm \frac{1}{2}$.

Plus the constrains form the Dirac Equation,
$$
U_2 =\frac{1}{E+m}\sigma\cdot p U_1
$$
To simplify these notation, we set $\vec p = p(\sin \theta\cos \phi, \sin \theta \sin \phi, \cos \theta)$,  
$$
\frac{1}{2}
\begin{bmatrix}
 \cos \theta & \sin \theta \mathrm e ^{-\mathrm i \phi}\\
\sin \theta\mathrm e ^{\mathrm i \phi} &-\cos \theta
\end{bmatrix}
\begin{bmatrix}
a\\
b
\end{bmatrix}
= \lambda 
\begin{bmatrix}
a\\
b
\end{bmatrix}
$$

$$
\frac{b}{a}
= \frac{2\lambda-\cos \theta}{\sin\theta}\mathrm e ^{\mathrm i \phi}
$$

When $\lambda = \frac{1}{2}$, we have
$$
\frac{b}{a}= \frac{\sin \frac {\theta}{2}\mathrm e^{\mathrm i \phi}}{\cos \frac{\theta}{2}}
$$
Thus
$$
u_\uparrow
=
\begin{bmatrix}
c\\
s \mathrm e ^{\mathrm i \phi}\\
\frac{p}{E+m} c\\
\frac{p}{E+m} s \mathrm e ^{\mathrm i \phi}\\
\end{bmatrix}, \quad
u_\downarrow
=
\begin{bmatrix}
-s\\
c \mathrm e ^{\mathrm i \phi}\\
\frac{p}{E+m} s\\
-\frac{p}{E+m} c \mathrm e ^{\mathrm i \phi}\\
\end{bmatrix}
$$

$$
v_\uparrow
=
\begin{bmatrix}
\frac{p}{E+m} s\\
-\frac{p}{E+m} c \mathrm e ^{\mathrm i \phi}\\
-s\\
c \mathrm e ^{\mathrm i \phi}\\
\end{bmatrix}, \quad
v_\downarrow
=
\begin{bmatrix}
\frac{p}{E+m} c\\
\frac{p}{E+m} s \mathrm e ^{\mathrm i \phi}\\
c\\
s \mathrm e ^{\mathrm i \phi}\\
\end{bmatrix}

$$

where $c = \cos \frac{\theta}{2}, s = \sin\frac{\theta}{2}$.

### Intrinsic parity for Dirac fermions

---

(TO BE CONTINUED)

---