---
layout: default
title: "Reading notes for Modern Particle Physics, Mark Thomson (Chapter 6)"
date: 2025-8-14
categories: [particle physics]
tags: [reading notes, particle physics]
---

Lots of key concepts are omitted... Complete them another day.

## Chapter 6 Electron-positron annihilation

### Calculations in perturbation theory

According in the discussion in Chapter 1, for QED process, the biggest contribution comes from the simplest Feynman diagram, as for the more vertex brings more $\alpha\approx\frac{1}{137}$ decays.

### Electron-positron annihilation

According to the Feynman diagram, for process $e^+e^-\to\mu^+\mu^-$:

![image-20250811114125762](https://raw.githubusercontent.com/stur007/img/main/img/202508111141323.png)

$$
-\mathrm i M =[\bar v_e(p_2)\{ie\gamma^\mu\} u_e(p_1)]\frac{-\mathrm  ig_{\mu\nu}}{q^2}[\overline u_\mu(p_3)\{\mathrm i e\gamma^\nu\} v_\mu(p_4)]
$$

i.e.,

$$
M = -\frac{e^2}{q^2}g_{\mu\nu}j_e^\mu j_\mu^\nu
$$

#### Spin sums

In the electron-positron collider, we cannot control the spin orientation of electrons and positrons. Considering the orthogonal of these states, we have, take one helicity for example

$$
|M_{RR}|^2 = (|M_{RR\to RR}|^2 + |M_{RL \to RR}|^2 +|M_{LR\to RR}|^2 + |M_{LL\to RR}|^2)
$$

and the average probability

$$
|M|^2 = \frac 1 4(|M_{RR}|^2 + |M_{RL}|^2+|M_{LR}|^2+|M_{LL}|^2)
$$

#### Helicity amplitudes

The geometry configuration for $e^-e^+\to\mu^-\mu^+$:

![image-20250811172734136](https://raw.githubusercontent.com/stur007/img/main/img/202508111727240.png)

For high-energy scenario, we have $m_e, m_\mu \approx 0$,

$$
p_1 = (E, 0, 0, E)\\
p_2 = (E, 0, 0, -E)\\
p_3 = (E, E\sin \theta, 0, E\cos\theta)\\
p_4 = (E, -E\sin \theta, 0, -E\cos \theta)
$$

And their helicity amplitudes

![image-20250811173309546](https://raw.githubusercontent.com/stur007/img/main/img/202508111733530.png)

![image-20250811173326515](https://raw.githubusercontent.com/stur007/img/main/img/202508111733515.png)

#### The muon and electron currents

Using the expression of currents, we have

![image-20250811173533161](https://raw.githubusercontent.com/stur007/img/main/img/202508111735275.png)

Apparently we can only take the conjugation and set $\theta \to 0$, then we have the non-zero electron currents

![image-20250811173734648](https://raw.githubusercontent.com/stur007/img/main/img/202508111737223.png)

#### The $e^-e^+\to \mu^-\mu^+$ cross section

With 

$$
M = -\frac{e^2}{q^2}g_{\mu\nu}j_e^\mu j_\mu^\nu
$$

add them up we get

$$
|M_{fi}|^2 = e^4 (1+\cos^2\theta)
$$

with

$$
\frac{\mathrm d \sigma}{\mathrm d^2 \Omega^*} =\frac{p_f^*}{64\pi^2(E_a^*+E_b^*)^2p_i^*}|M_{fi}|^2
$$

where $p_i^* = p_f^*$, $\sqrt s = E_a^*+E_b^*$, we have

$$
\frac{\mathrm d \sigma}{\mathrm d \Omega} = \frac{e^4(1+\cos^2\theta)}{64\pi^2s}
$$

Plus $\alpha = \frac{e^2}{4\pi }$, we have

$$
\frac{\mathrm d \sigma}{\mathrm d \Omega} = \frac{\alpha^2(1+\cos^2\theta)}{4s}
$$

Then the integral cross section

$$
\sigma = \frac{4\pi \alpha^2}{3s}
$$

#### Lorentz-invariant form

Apparently we can calculate the cross section in any other frame. 

Given that

![image-20250811175345140](https://raw.githubusercontent.com/stur007/img/main/img/202508111753428.png)

We have

$$
|M_{fi}|^2 =2e^4\frac{[(p_1\cdot p_3)^2+(p_1\cdot p_4)^2]}{(p_1\cdot p_2)^2}=  2e^4\frac{t^2+u^2}{s^2}
$$

### Spin in electron-positron annihilation

---

(TO BE CONTINUED)

### Chirality

The chirality property is denoted by the $\gamma^5$ matrix, 

$$
\gamma^5 = \gamma^0\gamma^1\gamma^2\gamma^3 = \begin{pmatrix}
0& I\\
I& 0
\end{pmatrix}
$$

Apparently it has the same property as other $\gamma$-matrices,

$$
{\gamma^5}^\dagger  = \gamma^5\\
(\gamma^5)^2 =1 \\
\gamma^5\gamma^\mu + \gamma^\mu \gamma^5 = 0
$$

And when $E \gg m$, the eigen vectors for H and h 

$$
u_\uparrow
=
N\begin{bmatrix}
c\\
s \mathrm e ^{\mathrm i \phi}\\
\frac{p}{E+m} c\\
\frac{p}{E+m} s \mathrm e ^{\mathrm i \phi}\\
\end{bmatrix}, \quad
u_\downarrow
=
N\begin{bmatrix}
-s\\
c \mathrm e ^{\mathrm i \phi}\\
\frac{p}{E+m} s\\
-\frac{p}{E+m} c \mathrm e ^{\mathrm i \phi}\\
\end{bmatrix},\quad
v_\uparrow
=
N\begin{bmatrix}
\frac{p}{E+m} s\\
-\frac{p}{E+m} c \mathrm e ^{\mathrm i \phi}\\
-s\\
c \mathrm e ^{\mathrm i \phi}\\
\end{bmatrix}, \quad
v_\downarrow
=
N\begin{bmatrix}
\frac{p}{E+m} c\\
\frac{p}{E+m} s \mathrm e ^{\mathrm i \phi}\\
c\\
s \mathrm e ^{\mathrm i \phi}\\
\end{bmatrix}
$$

come into 

$$
u_\uparrow \to u_R
=N
\begin{bmatrix}
c\\
s \mathrm e ^{\mathrm i \phi}\\
c\\
s \mathrm e ^{\mathrm i \phi}\\
\end{bmatrix}, \quad
u_\downarrow \to u_L
=N
\begin{bmatrix}
-s\\
c \mathrm e ^{\mathrm i \phi}\\
s\\
-c \mathrm e ^{\mathrm i \phi}\\
\end{bmatrix},\quad
v_\uparrow \to v_R
=N
\begin{bmatrix}
 s\\
- c \mathrm e ^{\mathrm i \phi}\\
-s\\
c \mathrm e ^{\mathrm i \phi}\\
\end{bmatrix}, \quad
v_\downarrow \to v_L
=N
\begin{bmatrix}
 c\\
s \mathrm e ^{\mathrm i \phi}\\
c\\
s \mathrm e ^{\mathrm i \phi}\\
\end{bmatrix}
$$

Thus we have

$$
\gamma^5 u_R = +u_R,\quad\gamma^5 u_L = - u_L, \quad \gamma^5 v_R = -v_R, \quad \gamma^5 v_L = +v_L 
$$

##### Chiral projection operators

These projection operators are defined by 

$$
P_R = \frac 1 2(1+\gamma^5) = \frac 1 2 
\begin{pmatrix}
I & I\\
I & I\\
\end{pmatrix}\\
P_L = \frac 1 2(1-\gamma^5) = \frac 1 2 
\begin{pmatrix}
I & -I\\
-I & I\\
\end{pmatrix}\\
$$

Thus

$$
P_Ru_R = u_R, P_Ru_L = 0, P_Rv_R = 0, P_Rv_L = v_L\\
P_Lu_R = 0, P_Lu_L = U_L, P_Lv_R = v_R, P_Lv_L = 0\\
$$

And

$$
u = a_Ru_R +a_Lu_L = P_Ru+P_Lu
$$

#### Chirality in QED

Let's consider the case that we encountered earlier, why $j^\mu_{RR} = j^\mu_{LL} = 0$?

For example,

$$
\begin{aligned}
\bar u_L 
&= u_L^\dagger \gamma_0 \\
&= (P_Lu_L)^\dagger \gamma_0\\
&= u_L^\dagger P_L^\dagger \gamma_0\\
&= u_L^\dagger \gamma_0P_R\\
&= \bar u_LP_R
\end{aligned}
$$

 And

$$
\begin{aligned}
\bar u_L\gamma^\mu u_R
&= \bar u_LP_R\gamma^0u_R\\
&= \bar u_L\gamma^0P_Lu_R\\
&= 0
\end{aligned}
$$

Thus we get the zero results by nature. 

#### Helicity and Chirality

When the condition $E \gg m $ isn't satisfied, we should keep in mind that the helicity and chirality are not the same idea, i.e.,

$$
u_\uparrow
=
N\begin{bmatrix}
c\\
s \mathrm e ^{\mathrm i \phi}\\
\kappa c\\
\kappa s \mathrm e ^{\mathrm i \phi}\\
\end{bmatrix}, \quad
u_\downarrow
=
N\begin{bmatrix}
-s\\
c \mathrm e ^{\mathrm i \phi}\\
\kappa s\\
-\kappa c \mathrm e ^{\mathrm i \phi}\\
\end{bmatrix},\quad
v_\uparrow
=
N\begin{bmatrix}
\kappa s\\
-\kappa c \mathrm e ^{\mathrm i \phi}\\
-s\\
c \mathrm e ^{\mathrm i \phi}\\
\end{bmatrix}, \quad
v_\downarrow
=
N\begin{bmatrix}
\kappa c\\
\kappa s \mathrm e ^{\mathrm i \phi}\\
c\\
s \mathrm e ^{\mathrm i \phi}\\
\end{bmatrix}
$$

where

$$
N = \sqrt {E+m}, \kappa =\frac {p}{E+m}
$$

we have

$$
u_\uparrow = P_Ru_\uparrow+P_Lu_\uparrow = \frac 1 2 (1+\kappa)u_R+\frac 1 2(1-\kappa)u_L
$$

> There's a trick (or mistake) in the book:
>
> This equation above make sense only when we set $u_R = \begin{bmatrix}\xi \\\xi \end{bmatrix}$ and $u_R = \begin{bmatrix}\xi \\-\xi \end{bmatrix}$ where $\xi = \begin{bmatrix}c \\ s\mathrm e ^{\mathrm i \phi}\end{bmatrix}$, which is in consistent with the setting above. 

![image-20250903182247808](https://raw.githubusercontent.com/stur007/img/main/img/202509031822351.png)

![image-20250903182312047](https://raw.githubusercontent.com/stur007/img/main/img/202509031823375.png)


### Trace techniques

---

(TO BE CONTINUED)

---
